<?xml version="1.0"?>


<!DOCTYPE rdf:RDF [
    <!ENTITY owl "http://www.w3.org/2002/07/owl#" >
    <!ENTITY dc "http://purl.org/dc/elements/1.1/" >
    <!ENTITY xsd "http://www.w3.org/2001/XMLSchema#" >
    <!ENTITY owl2xml "http://www.w3.org/2006/12/owl2-xml#" >
    <!ENTITY rdfs "http://www.w3.org/2000/01/rdf-schema#" >
    <!ENTITY rdf "http://www.w3.org/1999/02/22-rdf-syntax-ns#" >
]>


<rdf:RDF xmlns="http://purl.org/minim/minim#"
     xml:base="http://purl.org/minim/minim"
     xmlns:dc="http://purl.org/dc/elements/1.1/"
     xmlns:rdfs="http://www.w3.org/2000/01/rdf-schema#"
     xmlns:owl2xml="http://www.w3.org/2006/12/owl2-xml#"
     xmlns:owl="http://www.w3.org/2002/07/owl#"
     xmlns:xsd="http://www.w3.org/2001/XMLSchema#"
     xmlns:rdf="http://www.w3.org/1999/02/22-rdf-syntax-ns#">
    <owl:Ontology rdf:about="http://purl.org/minim/minim">
        <dc:creator>Graham Klyne</dc:creator>
        <rdfs:comment>Based on and adapted from ideas and a structure proposed by Matthew Gamble</rdfs:comment>
    </owl:Ontology>
    


    <!-- 
    ///////////////////////////////////////////////////////////////////////////////////////
    //
    // Annotation properties
    //
    ///////////////////////////////////////////////////////////////////////////////////////
     -->

    <owl:AnnotationProperty rdf:about="&dc;creator"/>
    <owl:AnnotationProperty rdf:about="http://purl.org/minim/minim#forPurpose">
        <rdfs:comment>Associates a descriptive label of the purpose the constraint serves to enable.

Note that a purpose is implicit in the constraint object itself, so the prupose is not treated as a separate resource, or given a separate URI.</rdfs:comment>
        <rdfs:domain rdf:resource="http://purl.org/minim/minim#Constraint"/>
    </owl:AnnotationProperty>
    <owl:AnnotationProperty rdf:about="&rdfs;comment"/>
    


    <!-- 
    ///////////////////////////////////////////////////////////////////////////////////////
    //
    // Datatypes
    //
    ///////////////////////////////////////////////////////////////////////////////////////
     -->

    


    <!-- 
    ///////////////////////////////////////////////////////////////////////////////////////
    //
    // Object Properties
    //
    ///////////////////////////////////////////////////////////////////////////////////////
     -->

    


    <!-- http://purl.org/minim/minim#aggregates -->

    <owl:ObjectProperty rdf:about="http://purl.org/minim/minim#aggregates">
        <rdfs:comment>This relation is true when the RO to which the subject RequirementRule is applied aggregates the indicated resource (via ore:aggregates), and the resource is physically present in the local RO structure.

The latter condition cannot be evaluated logically from the metadata alone, but requires some test of the RO environment.  Roughly, it means that if the RO is copied or cloned, the referenced resource becomes part of the new RO thus created.</rdfs:comment>
        <rdfs:domain rdf:resource="http://purl.org/minim/minim#RequirementRule"/>
        <rdfs:subPropertyOf rdf:resource="&owl;topObjectProperty"/>
    </owl:ObjectProperty>
    


    <!-- http://purl.org/minim/minim#derives -->

    <owl:ObjectProperty rdf:about="http://purl.org/minim/minim#derives">
        <rdfs:comment>Relates a requirement rule to a requirement for which it may generate a report.

Allows a requirement report to be inferred when all conditions on the subject RequirementRule are satisfied.

Thus, if S derivesRequirement R, and all conditions on S are satisfied, then S reports R can be inferred.</rdfs:comment>
        <rdfs:range rdf:resource="http://purl.org/minim/minim#Requirement"/>
        <rdfs:domain rdf:resource="http://purl.org/minim/minim#RequirementRule"/>
        <rdfs:subPropertyOf rdf:resource="&owl;topObjectProperty"/>
    </owl:ObjectProperty>
    


    <!-- http://purl.org/minim/minim#fullySatisfies -->

    <owl:ObjectProperty rdf:about="http://purl.org/minim/minim#fullySatisfies">
        <rdfs:range rdf:resource="http://purl.org/minim/minim#Model"/>
        <rdfs:domain rdf:resource="http://purl.org/minim/minim#Object"/>
        <rdfs:subPropertyOf rdf:resource="http://purl.org/minim/minim#nominallySatisfies"/>
    </owl:ObjectProperty>
    


    <!-- http://purl.org/minim/minim#hasConstraint -->

    <owl:ObjectProperty rdf:about="http://purl.org/minim/minim#hasConstraint">
        <rdfs:comment>Associates a constraint with a target resource.</rdfs:comment>
        <rdfs:range rdf:resource="http://purl.org/minim/minim#Constraint"/>
        <rdfs:subPropertyOf rdf:resource="&owl;topObjectProperty"/>
    </owl:ObjectProperty>
    


    <!-- http://purl.org/minim/minim#hasMayRequirement -->

    <owl:ObjectProperty rdf:about="http://purl.org/minim/minim#hasMayRequirement">
        <rdfs:subPropertyOf rdf:resource="http://purl.org/minim/minim#hasRequirement"/>
    </owl:ObjectProperty>
    


    <!-- http://purl.org/minim/minim#hasMustRequirement -->

    <owl:ObjectProperty rdf:about="http://purl.org/minim/minim#hasMustRequirement">
        <rdfs:subPropertyOf rdf:resource="http://purl.org/minim/minim#hasRequirement"/>
    </owl:ObjectProperty>
    


    <!-- http://purl.org/minim/minim#hasRequirement -->

    <owl:ObjectProperty rdf:about="http://purl.org/minim/minim#hasRequirement">
        <rdfs:domain rdf:resource="http://purl.org/minim/minim#Model"/>
        <rdfs:range rdf:resource="http://purl.org/minim/minim#Requirement"/>
        <rdfs:subPropertyOf rdf:resource="&owl;topObjectProperty"/>
    </owl:ObjectProperty>
    


    <!-- http://purl.org/minim/minim#hasShouldRequirement -->

    <owl:ObjectProperty rdf:about="http://purl.org/minim/minim#hasShouldRequirement">
        <rdfs:subPropertyOf rdf:resource="http://purl.org/minim/minim#hasRequirement"/>
    </owl:ObjectProperty>
    


    <!-- http://purl.org/minim/minim#isDerivedBy -->

    <owl:ObjectProperty rdf:about="http://purl.org/minim/minim#isDerivedBy">
        <rdfs:comment>Relates a requirement to a rule which may generate a report for that requirement.</rdfs:comment>
        <rdfs:domain rdf:resource="http://purl.org/minim/minim#Requirement"/>
        <rdfs:range rdf:resource="http://purl.org/minim/minim#RequirementRule"/>
        <owl:inverseOf rdf:resource="http://purl.org/minim/minim#derives"/>
        <rdfs:subPropertyOf rdf:resource="&owl;topObjectProperty"/>
    </owl:ObjectProperty>
    


    <!-- http://purl.org/minim/minim#isReportedBy -->

    <owl:ObjectProperty rdf:about="http://purl.org/minim/minim#isReportedBy">
        <rdfs:range rdf:resource="http://purl.org/minim/minim#Report"/>
        <rdfs:subPropertyOf rdf:resource="&owl;topObjectProperty"/>
    </owl:ObjectProperty>
    


    <!-- http://purl.org/minim/minim#minimallySatisfies -->

    <owl:ObjectProperty rdf:about="http://purl.org/minim/minim#minimallySatisfies">
        <rdfs:range rdf:resource="http://purl.org/minim/minim#Model"/>
        <rdfs:domain rdf:resource="http://purl.org/minim/minim#Object"/>
        <rdfs:subPropertyOf rdf:resource="http://purl.org/minim/minim#potentiallySatisfies"/>
    </owl:ObjectProperty>
    


    <!-- http://purl.org/minim/minim#nominallySatisfies -->

    <owl:ObjectProperty rdf:about="http://purl.org/minim/minim#nominallySatisfies">
        <rdfs:range rdf:resource="http://purl.org/minim/minim#Model"/>
        <rdfs:domain rdf:resource="http://purl.org/minim/minim#Object"/>
        <rdfs:subPropertyOf rdf:resource="http://purl.org/minim/minim#minimallySatisfies"/>
    </owl:ObjectProperty>
    


    <!-- http://purl.org/minim/minim#onResource -->

    <owl:ObjectProperty rdf:about="http://purl.org/minim/minim#onResource">
        <rdf:type rdf:resource="&owl;FunctionalProperty"/>
        <rdfs:comment>A resource to which a constraint is applied.  This mat be different from the target resource with whichthe constraint is associated.  For example, to create a particular file may require that the containing Research Object resource satisfies a given minimum information model.</rdfs:comment>
        <rdfs:domain rdf:resource="http://purl.org/minim/minim#Constraint"/>
        <rdfs:subPropertyOf rdf:resource="&owl;topObjectProperty"/>
    </owl:ObjectProperty>
    


    <!-- http://purl.org/minim/minim#potentiallySatisfies -->

    <owl:ObjectProperty rdf:about="http://purl.org/minim/minim#potentiallySatisfies">
        <rdfs:range rdf:resource="http://purl.org/minim/minim#Model"/>
        <rdfs:domain rdf:resource="http://purl.org/minim/minim#Object"/>
        <rdfs:subPropertyOf rdf:resource="&owl;topObjectProperty"/>
    </owl:ObjectProperty>
    


    <!-- http://purl.org/minim/minim#reports -->

    <owl:ObjectProperty rdf:about="http://purl.org/minim/minim#reports">
        <rdfs:domain rdf:resource="http://purl.org/minim/minim#Report"/>
        <rdfs:range rdf:resource="http://purl.org/minim/minim#Requirement"/>
        <owl:inverseOf rdf:resource="http://purl.org/minim/minim#isReportedBy"/>
        <rdfs:subPropertyOf rdf:resource="&owl;topObjectProperty"/>
    </owl:ObjectProperty>
    


    <!-- http://purl.org/minim/minim#toModel -->

    <owl:ObjectProperty rdf:about="http://purl.org/minim/minim#toModel">
        <rdf:type rdf:resource="&owl;FunctionalProperty"/>
        <rdfs:comment>Indicates a minimum information model that a constraint requires some resource to conform with.</rdfs:comment>
        <rdfs:domain rdf:resource="http://purl.org/minim/minim#Constraint"/>
        <rdfs:range rdf:resource="http://purl.org/minim/minim#Model"/>
        <rdfs:subPropertyOf rdf:resource="&owl;topObjectProperty"/>
    </owl:ObjectProperty>
    


    <!-- http://www.w3.org/2002/07/owl#topObjectProperty -->

    <owl:ObjectProperty rdf:about="&owl;topObjectProperty"/>
    


    <!-- 
    ///////////////////////////////////////////////////////////////////////////////////////
    //
    // Data properties
    //
    ///////////////////////////////////////////////////////////////////////////////////////
     -->

    


    <!-- http://purl.org/minim/minim#command -->

    <owl:DatatypeProperty rdf:about="http://purl.org/minim/minim#command">
        <rdfs:comment>Command to execute when evaluating SoftwareRequirementRule</rdfs:comment>
    </owl:DatatypeProperty>
    


    <!-- http://purl.org/minim/minim#forPurpose -->

    <owl:DatatypeProperty rdf:about="http://purl.org/minim/minim#forPurpose">
        <rdfs:comment>Associates a descriptive label of the purpose the constraint serves to enable.

Note that a purpose is implicit in the constraint object itself, so the prupose is not treated as a separate resource, or given a separate URI.</rdfs:comment>
        <rdfs:domain rdf:resource="http://purl.org/minim/minim#Constraint"/>
        <rdfs:subPropertyOf rdf:resource="&rdfs;label"/>
    </owl:DatatypeProperty>
    


    <!-- http://purl.org/minim/minim#response -->

    <owl:DatatypeProperty rdf:about="http://purl.org/minim/minim#response">
        <rdfs:comment>Command response expected when evaluating SoftwareRequirementRule</rdfs:comment>
    </owl:DatatypeProperty>
    


    <!-- http://www.w3.org/2000/01/rdf-schema#label -->

    <owl:DatatypeProperty rdf:about="&rdfs;label"/>
    


    <!-- 
    ///////////////////////////////////////////////////////////////////////////////////////
    //
    // Classes
    //
    ///////////////////////////////////////////////////////////////////////////////////////
     -->

    


    <!-- http://purl.org/minim/minim#Constraint -->

    <owl:Class rdf:about="http://purl.org/minim/minim#Constraint">
        <rdfs:comment xml:lang="en">Relates a Model (or Requirement?) to a target resource for some specific purpose.  The model may constrain some resource other than the target to which it is associated.</rdfs:comment>
    </owl:Class>
    


    <!-- http://purl.org/minim/minim#DataRequirementRule -->

    <owl:Class rdf:about="http://purl.org/minim/minim#DataRequirementRule">
        <owl:equivalentClass>
            <owl:Restriction>
                <owl:onProperty rdf:resource="http://purl.org/minim/minim#aggregates"/>
                <owl:someValuesFrom rdf:resource="http://purl.org/minim/minim#Object"/>
            </owl:Restriction>
        </owl:equivalentClass>
        <rdfs:subClassOf rdf:resource="http://purl.org/minim/minim#RequirementRule"/>
        <rdfs:comment>Requirement for specified data resource to be aggregated in RO</rdfs:comment>
    </owl:Class>
    


    <!-- http://purl.org/minim/minim#Model -->

    <owl:Class rdf:about="http://purl.org/minim/minim#Model">
        <owl:equivalentClass>
            <owl:Restriction>
                <owl:onProperty rdf:resource="http://purl.org/minim/minim#hasRequirement"/>
                <owl:someValuesFrom rdf:resource="http://purl.org/minim/minim#Requirement"/>
            </owl:Restriction>
        </owl:equivalentClass>
        <rdfs:comment xml:lang="en">Model denotes a Minimum Information Model.  Objects potentially satisfying the model are related by one of the *Satisfies properties.</rdfs:comment>
    </owl:Class>
    


    <!-- http://purl.org/minim/minim#Object -->

    <owl:Class rdf:about="http://purl.org/minim/minim#Object">
        <rdfs:comment xml:lang="en">Any object that reports a minim:Requirement.
The fact of so reporting a requirement may be triggered by a RequirementRule.</rdfs:comment>
    </owl:Class>
    


    <!-- http://purl.org/minim/minim#Report -->

    <owl:Class rdf:about="http://purl.org/minim/minim#Report">
        <owl:equivalentClass>
            <owl:Restriction>
                <owl:onProperty rdf:resource="http://purl.org/minim/minim#reports"/>
                <owl:someValuesFrom rdf:resource="http://purl.org/minim/minim#Requirement"/>
            </owl:Restriction>
        </owl:equivalentClass>
        <rdfs:subClassOf rdf:resource="http://purl.org/minim/minim#RequirementRule"/>
        <rdfs:comment xml:lang="en">Any object that reports a minim:Requirement.

minim:Reports are a subset of minim:RequirementRules that actually generate a report.</rdfs:comment>
    </owl:Class>
    


    <!-- http://purl.org/minim/minim#Requirement -->

    <owl:Class rdf:about="http://purl.org/minim/minim#Requirement">
        <rdfs:comment xml:lang="en">A requirement is an atomic reporting requirement for a minimum information model.</rdfs:comment>
    </owl:Class>
    


    <!-- http://purl.org/minim/minim#RequirementRule -->

    <owl:Class rdf:about="http://purl.org/minim/minim#RequirementRule">
        <owl:equivalentClass>
            <owl:Restriction>
                <owl:onProperty rdf:resource="http://purl.org/minim/minim#derives"/>
                <owl:someValuesFrom rdf:resource="http://purl.org/minim/minim#Requirement"/>
            </owl:Restriction>
        </owl:equivalentClass>
        <rdfs:subClassOf rdf:resource="http://purl.org/minim/minim#Object"/>
        <rdfs:comment xml:lang="en">A rule (of unspecified form or mechanism) that can be applied to
          determine that an object reports some requirement; i.e. is a minim:Report.
          One form of requirement rule is an OWL class definition of the form:
          Class(ReportClass); EquivalentClass(ReportClass, DefiningClass);
            SubclassOf(ReportClass, RestrictionOn(minimReports, SomeRequirement));</rdfs:comment>
    </owl:Class>
    


    <!-- http://purl.org/minim/minim#SoftwareRequirementRule -->

    <owl:Class rdf:about="http://purl.org/minim/minim#SoftwareRequirementRule">
        <owl:equivalentClass>
            <owl:Class>
                <owl:intersectionOf rdf:parseType="Collection">
                    <owl:Restriction>
                        <owl:onProperty rdf:resource="http://purl.org/minim/minim#command"/>
                        <owl:someValuesFrom rdf:resource="&xsd;string"/>
                    </owl:Restriction>
                    <owl:Restriction>
                        <owl:onProperty rdf:resource="http://purl.org/minim/minim#response"/>
                        <owl:someValuesFrom rdf:resource="&xsd;string"/>
                    </owl:Restriction>
                </owl:intersectionOf>
            </owl:Class>
        </owl:equivalentClass>
        <rdfs:subClassOf rdf:resource="http://purl.org/minim/minim#RequirementRule"/>
        <rdfs:comment>Requirement for specified software to be present in the operating environment</rdfs:comment>
    </owl:Class>
</rdf:RDF>



<!-- Generated by the OWL API (version 3.2.3.1824) http://owlapi.sourceforge.net -->

